WIP pre-remove numAlloc

Clap/Lang/FB/FB.lean
@@ -6,30 +6,35 @@ abbrev FB p := F p
 
 namespace FB
 
-def true (p : ℕ) : FB p := .c 1
-def false (p : ℕ) : FB p := .c 1
+def true (p : ℕ) [Fact (p ≥ 2)] : FB p := .c 1
+def false (p : ℕ) [Fact (p ≥ 2)] : FB p := .c 0
 
-def isValid {p : ℕ} (x : FB p) (varStore : ℕ → Option (ZMod p)) : Prop :=
+variable {p : ℕ} [Fact (p ≥ 2)]
+
+def isValid (x : FB p) (varStore : ℕ → Option (ZMod p)) : Prop :=
   x.eval varStore = .some 0 ∨
   x.eval varStore = .some 1
 
-def isAlwaysValid {p : ℕ} (x : FB p) : Prop :=
+def isAlwaysValid (x : FB p) : Prop :=
   ∀ varStore, x.isValid varStore
 
-def toBool {p : ℕ} (x : FB p) (varStore : ℕ → Option (ZMod p)) : Bool :=
+def toBool (x : FB p) (varStore : ℕ → Option (ZMod p)) : Bool :=
   x.eval varStore == .some 1
 
-def ofBool (p : ℕ) (x : Bool) : FB p :=
+def ofBool (p : ℕ) [Fact (p ≥ 2)] (x : Bool) : FB p :=
   if x then FB.true p else FB.false p
 
-lemma isValid_ofBool {p : ℕ} (b:Bool) : isAlwaysValid (FB.ofBool p b) := by
+lemma isValid_ofBool (b:Bool) : isAlwaysValid (FB.ofBool p b) := by
   unfold isAlwaysValid isValid FB.ofBool
   aesop
 
-def matchesUnaryFunction (p : ℕ) (spec_function: Bool → Bool) (function : FB p → FB p) : Prop :=
+def matchesUnaryFunction (p : ℕ) [Fact (p ≥ 2)] (spec_function: Bool → Bool) (function : FB p → FB p) : Prop :=
   ∀ (a: FB p) varStore, a.isValid varStore →
     (function a).eval varStore =
     (FB.ofBool p (spec_function (a.toBool varStore))).eval varStore
+
+def matchesConstraints (p : ℕ) [Fact (p ≥ 2)] (constraints: Prop) (function : Edsl.CircuitStateM p Unit) : Prop :=
+
 
 end FB
 
