Clap/Lang/FB/assert.lean
@@ -1,9 +1,12 @@
 import Clap.Lang.FB.FB
+import Clap.Lang.FB.not
 import Clap.eDSLState.Basic
 
 namespace Clap.Lang.FB
 
-def assert {p : ℕ} (a : FB p) : Edsl.CircuitStateM p Unit := do
+def assert {p : ℕ} [Fact (p ≥ 2)] (a : FB p) : Edsl.CircuitStateM p Unit := do
   Edsl.eq0 (not a)
+
+
 
 end Clap.Lang.FB
